\appendix\section{Appendix}

\subsection{Proof that simple matching dissimilarity is a metric}

Let \(\mathcal A\) be a categorical attribute space and let the dissimilarity
function, \(d : \mathcal A^2 \to \mathbb R\), be defined as
in~\eqref{eq:dissim}. Then \(d\) is a metric such that for all \(x, y, z \in
\mathcal A\):
\begin{multicols}{2}
    \begin{enumerate}[label=(\roman*)]
        \item \(d\left(x, y\right) \geq 0\)
        \item \(d\left(x, y\right) = 0 \iff x = y\)
        \item \(d\left(x, y\right) = d\left(y, x\right)\)
        \item \(d\left(x, y\right) + d\left(y, z\right) \geq
            d\left(x, z\right)\)
    \end{enumerate}
\end{multicols}

\begin{proof}
    Let \(\mathcal A\) be a categorical attribute space and consider any
    \(x,y,z \in \mathcal A\).
    \begin{enumerate}[label=(\roman*)]
        \item If \(x = y\), then \(x_j = y_j\) for all \(j = 1, \ldots, m\).
            Then it immediately follows that \(d(x,y) = 0\). Otherwise,
            \(\delta\left(x_j, y_j\right) = 1\) for at least one
            \(j = 1, \ldots, m\). Therefore, \(d(x, y) \geq 1\), as required.
        \item As above, if \(x = y\) then \(d(x, y) = 0\). Now consider any
            \(x, y \in \mathcal A\) such that \(d(x, y) = 0\). Then
            \(d(x, y) = 0 \iff \delta\left(x_j, y_j\right) = 0\) for all
            \(j = 1, \ldots, m \iff x_j = y_j\) for all
            \(j = 1, \ldots, m \iff x = y\), as required.
        \item This follows from the commutativity of equality in the definition
            of \(\delta\) in~\eqref{eq:dissim}:
            \[
                d(x, y) = \sum_{j=1}^{m}~\delta\left(x_j,~y_j\right)
                = \sum_{j=1}^{m}~\delta\left(y_j,~x_j\right)
                = d(y, x)
            \]
        \item Without ambiguity, let \(x, y, z\) each be represented as a set of
            its elements. Then an alternative form for \(d\) may be considered
            where \(d(x, y) = m - \abs*{x \cap y}\). With this, it is sufficient
            to show:
            \[
                \left(m - \abs*{x \cap y}\right)
                + \left(m - \abs*{y \cap z}\right)
                \geq m - \abs*{x \cap z}
            \]
            That is,
            \(\abs*{x \cap y} - \abs*{x \cap z} + \abs*{y \cap z} \leq m\). So,
            \[
                \begin{aligned}
                    \abs*{x \cap y} - \abs*{x \cap z} + \abs*{y \cap z}
                    & \leq
                    \abs*{x \cap \left(y \setminus z\right)} + \abs*{y \cap z}\\
                    & \leq
                    \abs*{y \setminus z} + \abs*{y \cap z}\\
                    & = \abs*{y} = m
                \end{aligned}
            \]
    \end{enumerate}

    Therefore, \(d\) satisfies conditions (i) \-- (iv) and is a metric.
\end{proof}
